hpaxos_time.thy
@@ -1,0 +1,1099 @@
+theory hpaxos_time
+imports Main hpaxos hpaxos_safety hpaxos_aux
+begin
+
+
+lemma Process1a_Enables_Action:
+  assumes "Enabled (Process1a a x) st"
+      and "is_safe a"
+      and "\<not> two_a_lrn_loop st a"
+      and "queued_msg st a = None"
+      and "x \<in> set (msgs st)"
+    shows "Enabled (AcceptorAction a) st"
+  using AcceptorAction_NotEnabled Process1a_Enabled assms(1) assms(2) assms(4) assms(5) by blast
+
+lemma no_acceptor_no_Process1a:
+  assumes "\<not> Enabled (AcceptorAction a) st"
+      and "is_safe a"
+      and "queued_msg st a = None"
+      and "x \<in> set (msgs st)"
+    shows "\<not> Enabled (Process1a a x) st"
+  using AcceptorAction_NotEnabled Process1a_Enables_Action assms(1) assms(2) assms(3) assms(4) by blast
+
+lemma Process1a_Req_known_msgs:
+  assumes "Spec f"
+      and "Process1a a x (f (i - 1)) (f i)"
+    shows "x \<in> set (known_msgs_acc (f i) a)"
+  by (metis Process1a.elims(2) Store_acc.elims(2) assms(2) in_set_member member_rec(1))
+
+
+
+lemma ProposerSendAction_Preserves_AcceptorAction:
+  assumes "ProposerSendAction st st2"
+      and "Enabled (AcceptorAction a) st"
+    shows "Enabled (AcceptorAction a) st2"
+proof -
+  have "ProposerSendAction st st2"
+    using assms(1) by blast
+  then show ?thesis
+    unfolding ProposerSendAction.simps
+  proof (elim exE)
+    fix blt
+    assume "Send1a blt st st2"
+    have "is_safe a"
+      using AcceptorAction_Enabled assms(2) by presburger
+    show ?thesis
+    proof (cases "two_a_lrn_loop st a")
+      case True
+      have "two_a_lrn_loop st2 a"
+        using True \<open>Send1a blt st st2\<close> by fastforce
+      show ?thesis
+        using AcceptorAction_Enabled \<open>is_safe a\<close> \<open>two_a_lrn_loop st2 a\<close> by blast
+    next
+      case False
+      have "\<not> two_a_lrn_loop st2 a"
+        using False \<open>Send1a blt st st2\<close> by fastforce
+      then show ?thesis
+      proof (cases "queued_msg st a = None")
+        case True
+        have "\<exists>m \<in> set (msgs st). Recv_acc st a m \<and> (type m = T1a \<or> type m = T1b)"
+          using AcceptorAction_NotEnabled False True \<open>is_safe a\<close> assms(2) by blast
+        then show ?thesis
+        proof (clarify)
+          fix m
+          assume "m \<in> set (msgs st)"
+             and "Recv_acc st a m"
+             and "type m = T1a \<or> type m = T1b"
+          have "m \<in> set (msgs st2)"
+            by (meson Next.elims(3) \<open>m \<in> set (msgs st)\<close> assms(1) next_msgs_preserved)
+          have "Recv_acc st2 a m"
+            by (smt (verit) Proper_acc.simps Recv_acc.elims(1) Send1a.simps WellFormed_monotone \<open>Recv_acc st a m\<close> \<open>Send1a blt st st2\<close> select_convs(2) select_convs(9) surjective update_convs(1))
+          have q0: "\<exists>m \<in> set (msgs st2). Recv_acc st2 a m \<and> (type m = T1a \<or> type m = T1b)"
+            using \<open>Recv_acc st2 a m\<close> \<open>m \<in> set (msgs st2)\<close> \<open>type m = T1a \<or> type m = T1b\<close> by blast
+          have q1: "(queued_msg st a = None \<and> (
+                      \<exists>m \<in> set (msgs st). Recv_acc st a m \<and> (type m = T1a \<or> type m = T1b)
+                    ))"
+            using True \<open>Recv_acc st a m\<close> \<open>m \<in> set (msgs st)\<close> \<open>type m = T1a \<or> type m = T1b\<close> by blast
+          show ?thesis
+            by (metis AcceptorAction_NotEnabled Send1a.elims(2) True \<open>Send1a blt st st2\<close> \<open>is_safe a\<close> ext_inject q0 surjective update_convs(1))
+        qed
+      next
+        case False
+        have "type (the (queued_msg st2 a)) = T1b \<and>
+               Recv_acc st2 a (the (queued_msg st2 a))"
+          by (smt (verit, ccfv_SIG) AcceptorAction_NotEnabled False Proper_acc.elims(1) Recv_acc.elims(1) Send1a.elims(2) WellFormed_monotone \<open>Send1a blt st st2\<close> \<open>\<not> two_a_lrn_loop st2 a\<close> \<open>is_safe a\<close> assms(2) ext_inject surjective update_convs(1))
+        show ?thesis
+          by (metis AcceptorAction_NotEnabled False Send1a.elims(1) \<open>Send1a blt st st2\<close> \<open>is_safe a\<close> \<open>type (the (queued_msg st2 a)) = T1b \<and> Recv_acc st2 a (the (queued_msg st2 a))\<close> select_convs(5) surjective update_convs(1))
+      qed
+    qed
+  qed
+qed
+
+lemma FakeAcceptorAction_Preserves_AcceptorAction:
+  assumes "FakeAcceptorAction st st2"
+      and "Enabled (AcceptorAction a) st"
+    shows "Enabled (AcceptorAction a) st2"
+proof -
+  have "FakeAcceptorAction st st2"
+    using assms(1) by blast
+  then show ?thesis
+    unfolding FakeAcceptorAction.simps
+  proof (clarify)
+    fix a2
+    have "is_safe a"
+      using AcceptorAction_Enabled assms(2) by presburger
+    assume "\<not> is_safe a2"
+    assume "FakeSend1b a2 st st2 \<or> FakeSend2a a2 st st2"
+    have "two_a_lrn_loop st2 a = two_a_lrn_loop st a"
+      by (metis FakeSend1b.elims(1) FakeSend2a.elims(2) \<open>FakeSend1b a2 st st2 \<or> FakeSend2a a2 st st2\<close> select_convs(6) surjective update_convs(1))
+    have "known_msgs_acc st2 a = known_msgs_acc st a"
+      by (metis FakeSend1b.simps FakeSend2a.simps \<open>FakeSend1b a2 st st2 \<or> FakeSend2a a2 st st2\<close> select_convs(2) surjective update_convs(1))
+    have "recent_msgs st2 a = recent_msgs st a"
+      by (metis FakeSend1b.elims(1) FakeSend2a.elims(2) \<open>FakeSend1b a2 st st2 \<or> FakeSend2a a2 st st2\<close> select_convs(4) surjective update_convs(1))
+    have "queued_msg st2 a = queued_msg st a"
+      by (metis FakeSend1b.elims(1) FakeSend2a.simps \<open>FakeSend1b a2 st st2 \<or> FakeSend2a a2 st st2\<close> ext_inject surjective update_convs(1))
+    show ?thesis
+    proof (cases "two_a_lrn_loop st a")
+      case True
+      show ?thesis
+        using AcceptorAction_NotEnabled True \<open>is_safe a\<close> \<open>two_a_lrn_loop st2 a = two_a_lrn_loop st a\<close> by blast
+    next
+      case False
+      show ?thesis
+      proof (cases "queued_msg st a = None")
+        case True
+        have "\<exists>m \<in> set (msgs st). Recv_acc st a m \<and> (type m = T1a \<or> type m = T1b)"
+          using AcceptorAction_NotEnabled False True \<open>is_safe a\<close> assms(2) by blast
+        then show ?thesis
+        proof (clarify)
+          fix m
+          assume "m \<in> set (msgs st)"
+             and "Recv_acc st a m"
+             and "type m = T1a \<or> type m = T1b"
+          have "m \<in> set (msgs st2)"
+            by (meson Next.elims(3) \<open>m \<in> set (msgs st)\<close> assms(1) next_msgs_preserved)
+          have "Recv_acc st2 a m"
+            by (metis MessageType.distinct(3) MessageType.distinct(5) Proper_acc.elims(1) Recv_acc.elims(2) Recv_acc.elims(3) WellFormed.elims(1) \<open>Recv_acc st a m\<close> \<open>known_msgs_acc st2 a = known_msgs_acc st a\<close> \<open>type m = T1a \<or> type m = T1b\<close>)
+          have q: "\<exists>m \<in> set (msgs st2). Recv_acc st2 a m \<and> (type m = T1a \<or> type m = T1b)"
+            using \<open>Recv_acc st2 a m\<close> \<open>m \<in> set (msgs st2)\<close> \<open>type m = T1a \<or> type m = T1b\<close> by blast
+          show ?thesis
+            by (metis AcceptorAction_NotEnabled True \<open>is_safe a\<close> \<open>queued_msg st2 a = queued_msg st a\<close> q)
+        qed
+      next
+        have TwoFalse: "\<not> two_a_lrn_loop st a"
+          by (simp add: False)
+        case False
+        have "type (the (queued_msg st2 a)) = T1b \<and>
+               Recv_acc st2 a (the (queued_msg st2 a))"
+          by (smt (verit) AcceptorAction_NotEnabled False MessageType.distinct(5) Proper_acc.elims(1) Recv_acc.elims(2) Recv_acc.elims(3) TwoFalse WellFormed.elims(1) \<open>is_safe a\<close> \<open>known_msgs_acc st2 a = known_msgs_acc st a\<close> \<open>queued_msg st2 a = queued_msg st a\<close> assms(2))
+        show ?thesis
+          using AcceptorAction_NotEnabled False \<open>is_safe a\<close> \<open>queued_msg st2 a = queued_msg st a\<close> \<open>type (the (queued_msg st2 a)) = T1b \<and> Recv_acc st2 a (the (queued_msg st2 a))\<close> by presburger
+      qed
+    qed
+  qed
+qed
+
+lemma LearnerAction_Preserves_AcceptorAction:
+  assumes "LearnerProcessAction st st2"
+      and "Enabled (AcceptorAction a) st"
+    shows "Enabled (AcceptorAction a) st2"
+proof -
+  have "LearnerProcessAction st st2"
+    using assms(1) by blast
+  then show ?thesis
+    unfolding LearnerProcessAction.simps LearnerAction.simps
+  proof (clarify)
+    fix ln
+    have "is_safe a"
+      using AcceptorAction_Enabled assms(2) by presburger
+    assume "(\<exists>m\<in>set (msgs st). LearnerRecv ln m st st2) \<or>
+            (\<exists>blt val. LearnerDecide ln blt val st st2)"
+    have "two_a_lrn_loop st2 a = two_a_lrn_loop st a"
+      by (metis (no_types, lifting) LearnerDecide.elims(1) LearnerRecv.elims(1) \<open>(\<exists>m\<in>set (msgs st). LearnerRecv ln m st st2) \<or> (\<exists>blt val. LearnerDecide ln blt val st st2)\<close> select_convs(6) surjective update_convs(3) update_convs(8))
+    have "known_msgs_acc st2 a = known_msgs_acc st a"
+      by (metis (no_types, lifting) LearnerDecide.elims(2) LearnerRecv.elims(2) \<open>(\<exists>m\<in>set (msgs st). LearnerRecv ln m st st2) \<or> (\<exists>blt val. LearnerDecide ln blt val st st2)\<close> select_convs(2) surjective update_convs(3) update_convs(8))
+    have "recent_msgs st2 a = recent_msgs st a"
+      by (metis (no_types, lifting) LearnerDecide.elims(1) LearnerRecv.elims(1) \<open>(\<exists>m\<in>set (msgs st). LearnerRecv ln m st st2) \<or> (\<exists>blt val. LearnerDecide ln blt val st st2)\<close> select_convs(4) surjective update_convs(3) update_convs(8))
+    have "queued_msg st2 a = queued_msg st a"
+      by (metis (no_types, lifting) LearnerDecide.elims(2) LearnerRecv.elims(2) \<open>(\<exists>m\<in>set (msgs st). LearnerRecv ln m st st2) \<or> (\<exists>blt val. LearnerDecide ln blt val st st2)\<close> ext_inject surjective update_convs(3) update_convs(8))
+    show ?thesis
+    proof (cases "two_a_lrn_loop st a")
+      case True
+      show ?thesis
+        using AcceptorAction_NotEnabled True \<open>is_safe a\<close> \<open>two_a_lrn_loop st2 a = two_a_lrn_loop st a\<close> by blast
+    next
+      case False
+      show ?thesis
+      proof (cases "queued_msg st a = None")
+        case True
+        have "\<exists>m \<in> set (msgs st). Recv_acc st a m \<and> (type m = T1a \<or> type m = T1b)"
+          using AcceptorAction_NotEnabled False True \<open>is_safe a\<close> assms(2) by blast
+        then show ?thesis
+        proof (clarify)
+          fix m
+          assume "m \<in> set (msgs st)"
+             and "Recv_acc st a m"
+             and "type m = T1a \<or> type m = T1b"
+          have "m \<in> set (msgs st2)"
+            by (meson Next.elims(3) \<open>m \<in> set (msgs st)\<close> assms(1) next_msgs_preserved)
+          have "Recv_acc st2 a m"
+            by (metis MessageType.distinct(3) MessageType.distinct(5) Proper_acc.elims(1) Recv_acc.elims(2) Recv_acc.elims(3) WellFormed.elims(1) \<open>Recv_acc st a m\<close> \<open>known_msgs_acc st2 a = known_msgs_acc st a\<close> \<open>type m = T1a \<or> type m = T1b\<close>)
+          have q: "\<exists>m \<in> set (msgs st2). Recv_acc st2 a m \<and> (type m = T1a \<or> type m = T1b)"
+            using \<open>Recv_acc st2 a m\<close> \<open>m \<in> set (msgs st2)\<close> \<open>type m = T1a \<or> type m = T1b\<close> by blast
+          show ?thesis
+            by (metis AcceptorAction_NotEnabled True \<open>is_safe a\<close> \<open>queued_msg st2 a = queued_msg st a\<close> q)
+        qed
+      next
+        have TwoFalse: "\<not> two_a_lrn_loop st a"
+          by (simp add: False)
+        case False
+        have "type (the (queued_msg st2 a)) = T1b \<and>
+               Recv_acc st2 a (the (queued_msg st2 a))"
+          by (smt (verit) AcceptorAction_NotEnabled False MessageType.distinct(5) Proper_acc.elims(1) Recv_acc.elims(2) Recv_acc.elims(3) TwoFalse WellFormed.elims(1) \<open>is_safe a\<close> \<open>known_msgs_acc st2 a = known_msgs_acc st a\<close> \<open>queued_msg st2 a = queued_msg st a\<close> assms(2))
+        show ?thesis
+          using AcceptorAction_NotEnabled False \<open>is_safe a\<close> \<open>queued_msg st2 a = queued_msg st a\<close> \<open>type (the (queued_msg st2 a)) = T1b \<and> Recv_acc st2 a (the (queued_msg st2 a))\<close> by presburger
+      qed
+    qed
+  qed
+qed
+
+lemma Other_Process1a_Preserves_AcceptorAction:
+  assumes "Process1a A m st st2"
+      and "A \<noteq> a"
+      and "Enabled (AcceptorAction a) st"
+    shows "Enabled (AcceptorAction a) st2"
+proof -
+  have "recent_msgs st a = recent_msgs st2 a"
+    by (metis Process1a.elims(2) assms(1) assms(2))
+  have "queued_msg st a = queued_msg st2 a"
+    by (metis Process1a.elims(2) assms(1) assms(2))
+  have "two_a_lrn_loop st a = two_a_lrn_loop st2 a"
+    by (metis Process1a.elims(2) assms(1))
+  have "\<forall>m. Recv_acc st a m = Recv_acc st2 a m"
+    by (smt (verit, best) Process1a.elims(2) Proper_acc.elims(1) Recv_acc.simps Store_acc.elims(2) WellFormed_monotone assms(1) assms(2))
+  then show ?thesis
+  proof (cases "two_a_lrn_loop st a")
+    case True
+    then show ?thesis
+      using AcceptorAction_Enabled \<open>two_a_lrn_loop st a = two_a_lrn_loop st2 a\<close> assms(3) by presburger
+  next
+    case False
+    then show ?thesis
+    proof (cases "queued_msg st2 a = None")
+      case True
+      have "\<exists>m \<in> set (msgs st2). Recv_acc st2 a m \<and> (type m = T1a \<or> type m = T1b)"
+        by (metis (full_types) AcceptorAction_Enabled False Process1a.elims(2) Send.elims(2) True \<open>\<forall>m. Recv_acc st a m = Recv_acc st2 a m\<close> \<open>queued_msg st a = queued_msg st2 a\<close> assms(1) assms(3) list.set_intros(2))
+      show ?thesis
+        using AcceptorAction_Enabled True \<open>\<exists>m\<in>set (msgs st2). Recv_acc st2 a m \<and> (type m = T1a \<or> type m = T1b)\<close> assms(3) by presburger
+    next
+      case False
+      have "queued_msg st a \<noteq> None"
+        by (simp add: False \<open>queued_msg st a = queued_msg st2 a\<close>)
+      then show ?thesis 
+        by (metis AcceptorAction_Enabled \<open>\<forall>m. Recv_acc st a m = Recv_acc st2 a m\<close> \<open>queued_msg st a = queued_msg st2 a\<close> \<open>two_a_lrn_loop st a = two_a_lrn_loop st2 a\<close> assms(3))
+    qed
+  qed
+qed
+
+lemma Other_Process1b_Preserves_AcceptorAction:
+  assumes "Process1b A m st st2"
+      and "A \<noteq> a"
+      and "Enabled (AcceptorAction a) st"
+    shows "Enabled (AcceptorAction a) st2"
+proof -
+  have "recent_msgs st a = recent_msgs st2 a"
+    using assms(1) assms(2) by fastforce
+  have "queued_msg st a = queued_msg st2 a"
+    using Process1b.simps assms(1) assms(2) by presburger
+  have "two_a_lrn_loop st a = two_a_lrn_loop st2 a"
+    by (smt (verit, ccfv_SIG) Process1b.simps assms(1) assms(2))
+  have "\<forall>m. Recv_acc st a m = Recv_acc st2 a m"
+    using assms(1) assms(2) by force
+  then show ?thesis
+  proof (cases "two_a_lrn_loop st a")
+    case True
+    then show ?thesis
+      using AcceptorAction_Enabled \<open>two_a_lrn_loop st a = two_a_lrn_loop st2 a\<close> assms(3) by presburger
+  next
+    case False
+    then show ?thesis
+    proof (cases "queued_msg st2 a = None")
+      case True
+      have "\<exists>m \<in> set (msgs st2). Recv_acc st2 a m \<and> (type m = T1a \<or> type m = T1b)"
+        using AcceptorAction_Enabled False Process1b.simps True \<open>\<forall>m. Recv_acc st a m = Recv_acc st2 a m\<close> \<open>queued_msg st a = queued_msg st2 a\<close> assms(1) assms(3) by presburger
+      show ?thesis
+        using AcceptorAction_Enabled True \<open>\<exists>m\<in>set (msgs st2). Recv_acc st2 a m \<and> (type m = T1a \<or> type m = T1b)\<close> assms(3) by presburger
+    next
+      case False
+      have "queued_msg st a \<noteq> None"
+        by (simp add: False \<open>queued_msg st a = queued_msg st2 a\<close>)
+      then show ?thesis 
+        by (metis AcceptorAction_Enabled \<open>\<forall>m. Recv_acc st a m = Recv_acc st2 a m\<close> \<open>queued_msg st a = queued_msg st2 a\<close> \<open>two_a_lrn_loop st a = two_a_lrn_loop st2 a\<close> assms(3))
+    qed
+  qed
+qed
+
+lemma Other_Process1bLearnerLoopStep_Preserves_AcceptorAction:
+  assumes "Process1bLearnerLoopStep A m st st2"
+      and "A \<noteq> a"
+      and "Enabled (AcceptorAction a) st"
+    shows "Enabled (AcceptorAction a) st2"
+proof -
+  have "recent_msgs st a = recent_msgs st2 a"
+    by (metis Process1bLearnerLoopStep.elims(2) assms(1) assms(2))
+  have "queued_msg st a = queued_msg st2 a"
+    by (metis Process1bLearnerLoopStep.simps assms(1))
+  have "two_a_lrn_loop st a = two_a_lrn_loop st2 a"
+    by (metis Process1bLearnerLoopStep.elims(2) assms(1))
+  have "\<forall>m. Recv_acc st a m = Recv_acc st2 a m"
+    by (smt (verit, ccfv_threshold) Process1bLearnerLoopStep.elims(2) Proper_acc.elims(1) Recv_acc.simps Store_acc.elims(2) WellFormed_monotone assms(1) assms(2))
+  then show ?thesis
+  proof (cases "two_a_lrn_loop st a")
+    case True
+    then show ?thesis
+      using AcceptorAction_Enabled \<open>two_a_lrn_loop st a = two_a_lrn_loop st2 a\<close> assms(3) by presburger
+  next
+    case False
+    then show ?thesis
+    proof (cases "queued_msg st2 a = None")
+      case True
+      have "\<exists>m \<in> set (msgs st2). Recv_acc st2 a m \<and> (type m = T1a \<or> type m = T1b)"
+        by (metis (full_types) AcceptorAction_Enabled False Process1bLearnerLoopStep.elims(2) Send.elims(2) True \<open>\<forall>m. Recv_acc st a m = Recv_acc st2 a m\<close> assms(1) assms(3) list.set_intros(2))
+      show ?thesis
+        using AcceptorAction_Enabled True \<open>\<exists>m\<in>set (msgs st2). Recv_acc st2 a m \<and> (type m = T1a \<or> type m = T1b)\<close> assms(3) by presburger
+    next
+      case False
+      have "queued_msg st a \<noteq> None"
+        by (simp add: False \<open>queued_msg st a = queued_msg st2 a\<close>)
+      then show ?thesis 
+        by (metis AcceptorAction_Enabled \<open>\<forall>m. Recv_acc st a m = Recv_acc st2 a m\<close> \<open>queued_msg st a = queued_msg st2 a\<close> \<open>two_a_lrn_loop st a = two_a_lrn_loop st2 a\<close> assms(3))
+    qed
+  qed
+qed
+
+lemma Other_Process1bLearnerLoopDone_Preserves_AcceptorAction:
+  assumes "Process1bLearnerLoopDone A st st2"
+      and "A \<noteq> a"
+      and "Enabled (AcceptorAction a) st"
+    shows "Enabled (AcceptorAction a) st2"
+proof -
+  have "recent_msgs st a = recent_msgs st2 a"
+    using assms(1) by auto
+  have "queued_msg st a = queued_msg st2 a"
+    using assms(1) by auto
+  have "two_a_lrn_loop st a = two_a_lrn_loop st2 a"
+    using assms(1) assms(2) by auto
+  have "\<forall>m. Recv_acc st a m = Recv_acc st2 a m"
+    using assms(1) by auto
+  then show ?thesis
+  proof (cases "two_a_lrn_loop st a")
+    case True
+    then show ?thesis
+      using AcceptorAction_Enabled \<open>two_a_lrn_loop st a = two_a_lrn_loop st2 a\<close> assms(3) by presburger
+  next
+    case False
+    then show ?thesis
+    proof (cases "queued_msg st2 a = None")
+      case True
+      have "\<exists>m \<in> set (msgs st). Recv_acc st2 a m \<and> (type m = T1a \<or> type m = T1b)"
+        using AcceptorAction_Enabled False True \<open>\<forall>m. Recv_acc st a m = Recv_acc st2 a m\<close> \<open>queued_msg st a = queued_msg st2 a\<close> assms(3) by presburger
+      then have "\<exists>m \<in> set (msgs st2). Recv_acc st2 a m \<and> (type m = T1a \<or> type m = T1b)"
+        using assms(1) ext_inject surjective update_convs(6) by auto
+      show ?thesis
+        using AcceptorAction_Enabled True \<open>\<exists>m\<in>set (msgs st2). Recv_acc st2 a m \<and> (type m = T1a \<or> type m = T1b)\<close> assms(3) by presburger
+    next
+      case False
+      have "queued_msg st a \<noteq> None"
+        by (simp add: False \<open>queued_msg st a = queued_msg st2 a\<close>)
+      then show ?thesis 
+        by (metis AcceptorAction_Enabled \<open>\<forall>m. Recv_acc st a m = Recv_acc st2 a m\<close> \<open>queued_msg st a = queued_msg st2 a\<close> \<open>two_a_lrn_loop st a = two_a_lrn_loop st2 a\<close> assms(3))
+    qed
+  qed
+qed
+
+
+lemma only_AcceptorAction_disables_AcceptorAction:
+  assumes "Next st st2"
+      and "Enabled (AcceptorAction a) st"
+      and "\<not> Enabled (AcceptorAction a) st2"
+    shows "AcceptorAction a st st2"
+proof -
+  have "AcceptorProcessAction st st2"
+    using FakeAcceptorAction_Preserves_AcceptorAction LearnerAction_Preserves_AcceptorAction Next.simps ProposerSendAction_Preserves_AcceptorAction assms(1) assms(2) assms(3) by blast
+  then show ?thesis
+    unfolding AcceptorProcessAction.simps
+  proof (clarify)
+    fix A
+    assume "AcceptorAction A st st2"
+    have "a = A"
+      by (metis (full_types) AcceptorAction.elims(2) Other_Process1a_Preserves_AcceptorAction Other_Process1bLearnerLoopDone_Preserves_AcceptorAction Other_Process1bLearnerLoopStep_Preserves_AcceptorAction Other_Process1b_Preserves_AcceptorAction Process1bLearnerLoop.simps \<open>AcceptorAction A st st2\<close> assms(2) assms(3))
+    then show ?thesis
+      using \<open>AcceptorAction A st st2\<close> by blast 
+  qed
+qed
+
+
+
+lemma Process1b_Not_Process1bLearnerLoopStep:
+  assumes "Process1b a ln st st2"
+  shows "\<not> Process1bLearnerLoopStep a2 ln2 st st2"
+  by (smt (z3) Process1b.elims(1) Process1bLearnerLoopStep.elims(1) Send.elims(1) assms not_Cons_self)
+
+lemma Process1b_Not_Process1a:
+  assumes "Process1b a ln st st2"
+  shows "\<not> Process1a a2 ln2 st st2"
+  by (smt (z3) MessageType.simps(2) Process1a.simps Process1b.elims(1) assms list.distinct(1) list.inject not_Cons_self)
+
+lemma Process1a_Not_Process1bLearnerLoopDone:
+  assumes "Process1a a ln st st2"
+  shows "\<not> Process1bLearnerLoopDone a2 st st2"
+  by (smt (verit, best) Process1a.elims(2) Process1bLearnerLoopDone.elims(1) Send.elims(1) assms ext_inject not_Cons_self2 surjective update_convs(6))
+
+lemma Process1b_Not_Process1bLearnerLoopDone:
+  assumes "Process1b a ln st st2"
+  shows "\<not> Process1bLearnerLoopDone a2 st st2"
+  by (metis (mono_tags, lifting) Process1b.elims(2) Process1bLearnerLoopDone.elims(2) Store_acc.simps assms not_Cons_self select_convs(2) surjective update_convs(6))
+
+
+lemma Process1a_Not_ProposerSendAction :
+  assumes "Process1a a m st st2"
+    shows "\<not> ProposerSendAction st st2"
+  by (metis (no_types, lifting) Process1a.elims(2) ProposerSendAction.elims(2) Send1a.elims(2) Store_acc.elims(2) assms not_Cons_self2 select_convs(2) surjective update_convs(1))
+
+lemma Process1a_Not_LearnerProcessAction :
+  assumes "Process1a a m st st2"
+    shows "\<not> LearnerProcessAction st st2"
+  by (smt (verit) LearnerProcessAction.elims LearnerAction.elims(2) LearnerDecide.elims(2) LearnerRecv.elims(2) Process1a.elims(2) Send.elims(1) assms ext_inject not_Cons_self2 surjective update_convs(3) update_convs(8))
+
+lemma Process1a_Not_FakeAcceptorAction :
+  assumes "Process1a a m st st2"
+    shows "\<not> FakeAcceptorAction st st2"
+  by (metis FakeAcceptorAction.simps FakeSend1b.elims(1) FakeSend2a.simps Process1a.elims(2) Store_acc.elims(2) assms not_Cons_self2 select_convs(2) surjective update_convs(1))
+
+lemma Process1a_Next_Implies_AcceptorAction:
+  assumes "Next st st2"
+      and "Process1a a m st st2"
+    shows "AcceptorAction a st st2"
+proof -
+  have "AcceptorProcessAction st st2"
+    using Next.simps Process1a_Not_FakeAcceptorAction Process1a_Not_LearnerProcessAction Process1a_Not_ProposerSendAction assms(1) assms(2) by blast
+  then show ?thesis
+    unfolding AcceptorProcessAction.simps
+  proof (elim exE)
+    fix a2
+    assume "AcceptorAction a2 st st2"
+    have "\<exists>m \<in> set (msgs st). Process1a a2 m st st2 \<or> Process1b a2 m st st2"
+      by (metis AcceptorAction.simps Process1a_Not_Process1bLearnerLoopDone Process1a_Not_Process1bLearnerLoopStep Process1bLearnerLoop.elims(1) Process1b_Not_Process1a \<open>AcceptorAction a2 st st2\<close> assms(2))
+    have "Process1a a2 m st st2"
+      by (metis Process1a.elims(2) Process1b_Not_Process1a Store_acc.elims(2) \<open>\<exists>m\<in>set (msgs st). Process1a a2 m st st2 \<or> Process1b a2 m st st2\<close> assms(2) not_Cons_self2)
+    have "a = a2"
+      by (metis Process1a.simps Store_acc.elims(2) \<open>Process1a a2 m st st2\<close> assms(2) not_Cons_self)
+    then show ?thesis
+      using \<open>AcceptorAction a2 st st2\<close> by blast
+  qed
+qed
+
+
+
+
+
+lemma Process1B_Not_ProposerSendAction :
+  assumes "Process1b a m st st2"
+    shows "\<not> ProposerSendAction st st2"
+proof -
+  have "recent_msgs st2 a \<noteq> recent_msgs st a"
+    using assms by auto
+  then show ?thesis
+    by force
+qed
+
+lemma Process1b_Not_LearnerProcessAction :
+  assumes "Process1b a m st st2"
+    shows "\<not> LearnerProcessAction st st2"
+proof -
+  have "recent_msgs st2 a \<noteq> recent_msgs st a"
+    using assms by auto
+  then show ?thesis
+    by force
+qed
+
+lemma Process1b_Not_FakeSend1b :
+  assumes "Process1b a m st st2"
+    shows "\<not> FakeSend1b a2 st st2"
+  by (smt (z3) FakeSend1b.elims(1) Process1b.elims(1) assms not_Cons_self select_convs(4) surjective update_convs(1))
+
+lemma Process1b_Not_FakeSend2a :
+  assumes "Process1b a m st st2"
+    shows "\<not> FakeSend2a a2 st st2"
+proof -
+  have "recent_msgs st2 a \<noteq> recent_msgs st a"
+    using assms by auto
+  then show ?thesis
+    by (metis FakeSend2a.simps select_convs(4) surjective update_convs(1))
+qed
+
+lemma Process1b_Not_FakeAcceptorAction :
+  assumes "Process1b a m st st2"
+    shows "\<not> FakeAcceptorAction st st2"
+  using FakeAcceptorAction.simps Process1b_Not_FakeSend1b Process1b_Not_FakeSend2a assms by presburger
+
+lemma Process1b_Next_Implies_AcceptorAction:
+  assumes "Next st st2"
+      and "Process1b a m st st2"
+    shows "AcceptorAction a st st2"
+proof -
+  have "AcceptorProcessAction st st2"
+    using Next.simps Process1B_Not_ProposerSendAction Process1b_Not_FakeAcceptorAction Process1b_Not_LearnerProcessAction assms(1) assms(2) by blast
+  then show ?thesis
+    unfolding AcceptorProcessAction.simps
+    proof (elim exE)
+    fix a2
+    assume "AcceptorAction a2 st st2"
+    then show ?thesis
+    proof (cases "queued_msg st a = None")
+      case True
+      then show ?thesis
+        by (metis AcceptorAction.simps Process1b.elims(2) Process1bLearnerLoop.elims(2) Process1b_Not_Process1a Process1b_Not_Process1bLearnerLoopDone Process1b_Not_Process1bLearnerLoopStep \<open>AcceptorAction a2 st st2\<close> assms(2) not_Cons_self)
+    next
+      case False
+      then show ?thesis
+      proof -
+        have f1: "\<And>aa. aa \<noteq> a \<or> queued_msg st2 aa = None"
+          by (meson Process1b.elims(2) assms(2))
+        have "\<forall>s a sa. \<exists>p. \<forall>sb aa sc ab sd se. (\<not> two_a_lrn_loop sb aa \<or> \<not> AcceptorAction aa sb sc \<or> Process1bLearnerLoop aa sb sc) \<and> (\<not> AcceptorAction ab sd se \<or> two_a_lrn_loop sd ab \<or> queued_msg sd ab = None \<or> Process1b ab (the (queued_msg sd ab)) sd se) \<and> (queued_msg s a \<noteq> None \<or> \<not> AcceptorAction a s sa \<or> two_a_lrn_loop s a \<or> Process1b a p s sa \<or> Process1a a p s sa)"
+          using AcceptorAction.simps by blast
+        then obtain pp :: "State \<Rightarrow> Acceptor \<Rightarrow> State \<Rightarrow> PreMessage" where
+          f2: "\<And>s a sa aa sb sc sd ab se. (\<not> two_a_lrn_loop s a \<or> \<not> AcceptorAction a s sa \<or> Process1bLearnerLoop a s sa) \<and> (\<not> AcceptorAction aa sb sc \<or> two_a_lrn_loop sb aa \<or> queued_msg sb aa = None \<or> Process1b aa (the (queued_msg sb aa)) sb sc) \<and> (queued_msg sd ab \<noteq> None \<or> \<not> AcceptorAction ab sd se \<or> two_a_lrn_loop sd ab \<or> Process1b ab (pp sd ab se) sd se \<or> Process1a ab (pp sd ab se) sd se)"
+          by metis
+        then have "\<not> two_a_lrn_loop st a2"
+          by (metis (no_types) Process1bLearnerLoop.simps Process1b_Not_Process1bLearnerLoopDone Process1b_Not_Process1bLearnerLoopStep \<open>AcceptorAction a2 st st2\<close> assms(2))
+        then have "Process1a a2 (pp st a2 st2) st st2 \<or> a2 = a"
+          using f2 f1 by (metis (full_types) False Process1b.elims(2) \<open>AcceptorAction a2 st st2\<close>)
+        then have "a2 = a"
+          using f1 by (metis (no_types) False Process1a.elims(2))
+        then show ?thesis
+          using \<open>AcceptorAction a2 st st2\<close> by force
+      qed
+    qed
+  qed
+qed
+
+
+
+
+lemma Process1bLearnerLoopDone_Not_ProposerSendAction :
+  assumes "Process1bLearnerLoopDone a st st2"
+    shows "\<not> ProposerSendAction st st2"
+  by (metis (no_types, lifting) Process1bLearnerLoopDone.elims(1) ProposerSendAction.elims(2) Send1a.elims(2) assms not_Cons_self select_convs(1) surjective update_convs(1) update_convs(6))
+
+lemma Process1bLearnerLoopDone_Not_LearnerRecv :
+  assumes "Process1bLearnerLoopDone a st st2"
+    shows "\<not> LearnerRecv ln m st st2"
+  by (smt (verit, best) LearnerRecv.elims(2) Process1bLearnerLoopDone.elims(1) assms ext_inject not_Cons_self2 surjective update_convs(3) update_convs(6))
+
+lemma Process1bLearnerLoopDone_Not_LearnerDecide :
+  assumes "Process1bLearnerLoopDone a st st2"
+      and "st \<noteq> st2"
+    shows "\<not> LearnerDecide ln blt val st st2"
+  by (metis (no_types, lifting) LearnerDecide.elims(1) Process1bLearnerLoopDone.elims(2) assms(1) assms(2) select_convs(8) surjective update_convs(6) update_convs(8))
+
+lemma Process1bLearnerLoopDone_Not_LearnerProcessAction :
+  assumes "Process1bLearnerLoopDone a st st2"
+      and "st \<noteq> st2"
+    shows "\<not> LearnerProcessAction st st2"
+  by (meson LearnerProcessAction.elims LearnerAction.elims(2) Process1bLearnerLoopDone_Not_LearnerDecide Process1bLearnerLoopDone_Not_LearnerRecv assms)
+
+lemma Process1bLearnerLoopDone_Not_FakeSend1b :
+  assumes "Process1bLearnerLoopDone a st st2"
+    shows "\<not> FakeSend1b a2 st st2"
+  by (smt (verit, ccfv_threshold) FakeSend1b.elims(1) Process1bLearnerLoopDone.elims(2) assms ext_inject not_Cons_self2 surjective update_convs(1) update_convs(6))
+
+lemma Process1bLearnerLoopDone_Not_FakeSend2a :
+  assumes "Process1bLearnerLoopDone a st st2"
+    shows "\<not> FakeSend2a a2 st st2"
+  by (smt (verit, ccfv_threshold) FakeSend2a.elims(2) Process1bLearnerLoopDone.simps assms ext_inject not_Cons_self2 surjective update_convs(1) update_convs(6))
+
+lemma Process1bLearnerLoopDone_Not_FakeAcceptorAction :
+  assumes "Process1bLearnerLoopDone a st st2"
+    shows "\<not> FakeAcceptorAction st st2"
+  using FakeAcceptorAction.simps Process1bLearnerLoopDone_Not_FakeSend1b Process1bLearnerLoopDone_Not_FakeSend2a assms by blast
+
+lemma Process1bLearnerLoopDone_Next_Implies_AcceptorAction:
+  assumes "Next st st2"
+      and "Process1bLearnerLoopDone a st st2"
+      and "st \<noteq> st2"
+    shows "AcceptorAction a st st2"
+proof -
+  have "\<not> two_a_lrn_loop st2 a"
+    using assms(2) by auto
+  have "two_a_lrn_loop st \<noteq> two_a_lrn_loop st2"
+    using assms(2) assms(3) by fastforce
+  have "\<forall>A. A \<noteq> a \<longrightarrow> two_a_lrn_loop st A = two_a_lrn_loop st2 A"
+    using assms(2) by auto
+  have "two_a_lrn_loop st a \<noteq> two_a_lrn_loop st2 a"
+    using \<open>\<forall>A. A \<noteq> a \<longrightarrow> two_a_lrn_loop st A = two_a_lrn_loop st2 A\<close> \<open>two_a_lrn_loop st \<noteq> two_a_lrn_loop st2\<close> by auto
+  have "two_a_lrn_loop st a"
+    using \<open>\<not> two_a_lrn_loop st2 a\<close> \<open>two_a_lrn_loop st a \<noteq> two_a_lrn_loop st2 a\<close> by blast
+  have "AcceptorProcessAction st st2"
+    using Next.simps Process1bLearnerLoopDone_Not_FakeAcceptorAction Process1bLearnerLoopDone_Not_LearnerProcessAction Process1bLearnerLoopDone_Not_ProposerSendAction assms(1) assms(2) assms(3) by blast
+  then show ?thesis
+    unfolding AcceptorProcessAction.simps
+  proof (elim exE)
+    fix a2
+    assume "AcceptorAction a2 st st2"
+    have "Process1bLearnerLoopDone a2 st st2"
+      by (metis AcceptorAction.simps Process1a_Not_Process1bLearnerLoopDone Process1bLearnerLoop.simps Process1bLearnerLoopStep.elims(2) Process1b_Not_Process1bLearnerLoopDone \<open>AcceptorAction a2 st st2\<close> \<open>two_a_lrn_loop st \<noteq> two_a_lrn_loop st2\<close> assms(2))
+    have "a = a2"
+      using \<open>Process1bLearnerLoopDone a2 st st2\<close> \<open>\<not> two_a_lrn_loop st2 a\<close> \<open>two_a_lrn_loop st a\<close> surjective by fastforce
+    show ?thesis
+      using \<open>AcceptorAction a2 st st2\<close> \<open>a = a2\<close> by blast
+  qed
+qed
+
+
+lemma Process1a_not_looping_Next:
+  assumes "Next st st2"
+  shows "(\<exists>m\<in>set (msgs st). Process1a a m st st2) \<longrightarrow> \<not> two_a_lrn_loop st a"
+  by (meson AcceptorAction.elims(2) Process1a_Next_Implies_AcceptorAction Process1a_Not_Process1bLearnerLoopDone Process1a_Not_Process1bLearnerLoopStep Process1bLearnerLoop.elims(2) assms)
+
+lemma Process1a_not_looping:
+  assumes "Spec f"
+  shows "(\<exists>m\<in>set (msgs (f i)). Process1a a m (f i) (f (1 + i))) \<longrightarrow> \<not> two_a_lrn_loop (f i) a"
+proof (induction i)
+  case 0
+  then show ?case
+    by (metis Init.simps Spec.simps assms select_convs(6))
+next
+  case (Suc i)
+  then show ?case
+    by (metis AcceptorAction.elims(2) Process1a.elims(2) Process1a_Next_Implies_AcceptorAction Process1a_Not_Process1bLearnerLoopDone Process1a_Not_Process1bLearnerLoopStep Process1bLearnerLoop.elims(2) Send.elims(2) Spec.elims(2) assms not_Cons_self plus_1_eq_Suc)
+qed
+
+lemma no_queue_during_loop_Next:
+  assumes "Next st st2" 
+      and "two_a_lrn_loop st a \<longrightarrow> queued_msg st a = None"
+      and "(\<exists>m\<in>set (msgs st). Process1a a m st st2) \<longrightarrow> \<not> two_a_lrn_loop st a"
+    shows "two_a_lrn_loop st2 a \<longrightarrow> queued_msg st2 a = None"
+proof -
+  have css: "ProposerSendAction st st2 \<or>
+        (\<exists>A :: Acceptor. is_safe A
+                    \<and> queued_msg st A = None 
+                    \<and> (\<exists>m \<in> set (msgs st). Process1a A m st st2)) \<or>
+        (\<exists>A :: Acceptor. is_safe A
+                      \<and> queued_msg st A \<noteq> None 
+                      \<and> Process1b A (the (queued_msg st A)) st st2) \<or>
+        (\<exists>A :: Acceptor. is_safe A
+                      \<and> queued_msg st A = None 
+                      \<and> (\<exists>m \<in> set (msgs st). Process1b A m st st2)) \<or>
+        (\<exists>A :: Acceptor. is_safe A
+                      \<and> two_a_lrn_loop st A 
+                      \<and> (\<exists>l :: Learner. Process1bLearnerLoopStep A l st st2)) \<or>
+        (\<exists>A :: Acceptor. is_safe A
+                      \<and> two_a_lrn_loop st A 
+                      \<and> Process1bLearnerLoopDone A st st2) \<or>
+        LearnerProcessAction st st2 \<or>
+        (\<exists>A :: Acceptor. \<not> (is_safe A)
+                      \<and> FakeSend1b A st st2) \<or>
+        (\<exists>A :: Acceptor. \<not> (is_safe A)
+                      \<and> FakeSend2a A st st2)
+        "
+        using assms next_split by presburger
+    then show ?thesis
+    proof (elim disjE)
+      assume "ProposerSendAction st st2"
+      then show ?thesis
+        using assms(2) by auto
+    next
+      assume "\<exists>A. is_safe A \<and>
+                queued_msg st A = None \<and>
+                (\<exists>m\<in>set (msgs st).
+                    Process1a A m st st2)"
+      then show ?thesis
+      proof (clarify)
+        fix A m
+        assume "is_safe A"
+           and "queued_msg st A = None"
+           and "m \<in> set (msgs st)"
+           and "Process1a A m st st2"
+           and "two_a_lrn_loop st2 a"
+        then show "queued_msg st2 a = None"
+        proof (cases "A = a")
+          case True
+          define new1b where "new1b = M1b A (m # recent_msgs st A)"
+          show ?thesis
+          proof (cases "WellFormed st new1b")
+            case True
+            then show ?thesis
+              by (metis Process1a.elims(2) \<open>\<exists>A. is_safe A \<and> queued_msg st A = None \<and> (\<exists>m\<in>set (msgs st). Process1a A m st st2)\<close> \<open>two_a_lrn_loop st2 a\<close> assms(2) assms(3))
+          next
+            case False
+            then show ?thesis
+              by (metis Process1a.elims(2) True \<open>Process1a A m st st2\<close> \<open>queued_msg st A = None\<close> new1b_def)
+          qed
+        next
+          case False
+          then show ?thesis
+            by (metis Process1a.elims(2) \<open>Process1a A m st st2\<close> \<open>two_a_lrn_loop st2 a\<close> assms(2))
+        qed
+      qed
+    next
+      assume "\<exists>A :: Acceptor. is_safe A
+                        \<and> queued_msg st A \<noteq> None 
+                        \<and> Process1b A (the (queued_msg st A)) st st2"
+      then show ?thesis
+        unfolding Process1b.simps
+        by (metis (no_types, lifting) assms(2))
+    next
+      assume "\<exists>A :: Acceptor. is_safe A
+                  \<and> queued_msg st A = None 
+                  \<and> (\<exists>m \<in> set (msgs st). Process1b A m st st2)"
+      then show ?thesis
+        unfolding Process1b.simps
+        by (metis assms(2))
+    next
+      assume "\<exists>A :: Acceptor. is_safe A
+                        \<and> two_a_lrn_loop st A 
+                        \<and> (\<exists>l :: Learner. Process1bLearnerLoopStep A l st st2)"
+      then show ?thesis
+        by (metis Process1bLearnerLoopStep.elims(2) assms(2))
+    next
+      assume "\<exists>A. is_safe A \<and>
+        two_a_lrn_loop st A \<and>
+        Process1bLearnerLoopDone A st st2"
+      then show ?thesis
+      proof (clarify)
+        fix A
+        assume "is_safe A"
+           and "two_a_lrn_loop st A"
+           and "Process1bLearnerLoopDone A st st2"
+           and "two_a_lrn_loop st2 a"
+        then show "queued_msg st2 a = None"
+        proof (cases "A = a")
+          case True
+          then show ?thesis
+            using \<open>Process1bLearnerLoopDone A st st2\<close> \<open>two_a_lrn_loop st A\<close> assms(2) by auto
+        next
+          case False
+          then show ?thesis
+            using \<open>Process1bLearnerLoopDone A st st2\<close> \<open>two_a_lrn_loop st2 a\<close> assms(2) by auto
+        qed
+      qed
+    next
+      assume "LearnerProcessAction st st2"
+      then show ?thesis
+        by (smt (verit, del_insts) LearnerProcessAction.elims LearnerAction.elims(2) LearnerDecide.simps LearnerRecv.elims(2) assms(2) ext_inject surjective update_convs(3) update_convs(8))
+    next
+      assume "\<exists>A. \<not> is_safe A \<and> FakeSend1b A st st2"
+      show ?thesis
+        by (metis FakeSend1b.elims(1) \<open>\<exists>A. \<not> is_safe A \<and> FakeSend1b A st st2\<close> assms(2) ext_inject surjective update_convs(1))
+    next
+      assume "\<exists>A. \<not> is_safe A \<and> FakeSend2a A st st2"
+      then show ?thesis
+        by (metis FakeSend2a.simps assms(2) ext_inject surjective update_convs(1))
+    qed
+qed
+
+lemma no_queue_during_loop:
+  assumes "Spec f"
+  shows "two_a_lrn_loop (f i) a \<longrightarrow> queued_msg (f i) a = None"
+proof (induction i)
+  case 0
+  then show ?case
+    by (metis Init.elims Spec.elims(2) assms ext_inject surjective)
+next
+  case (Suc i)
+  then show ?case
+    by (metis Process1a_not_looping Spec.elims(2) assms no_queue_during_loop_Next plus_1_eq_Suc)
+qed
+
+lemma ballot_present:
+  shows "M1a b \<in> set l \<longrightarrow> b \<in> (Get1a ` set l)"
+proof (induction l)
+  case Nil
+  then show ?case 
+    by simp
+next
+  case (Cons a l)
+  then show ?case
+  proof (cases "a = M1a b")
+    case True
+    have "b \<in> Get1a ` set (M1a b # l)"
+      by auto
+    show ?thesis
+      using True \<open>b \<in> Get1a ` set (M1a b # l)\<close> by presburger
+  next
+    case False
+    then show ?thesis
+      using local.Cons by auto
+  qed
+qed
+
+lemma new_bal_unknown:
+  assumes "\<forall>a \<in> Q. the (MaxBalO st a) < bal x"
+      and "type x = T1a"
+    shows "\<forall>a \<in> Q. x \<notin> set (known_msgs_acc st a)"
+proof (clarify)
+  fix a
+  assume "a \<in> Q"
+     and "x \<in> set (known_msgs_acc st a)"
+  then show False
+  proof (cases "known_msgs_acc st a")
+    case Nil
+    then show ?thesis
+      using \<open>x \<in> set (known_msgs_acc st a)\<close> by auto
+  next
+    case (Cons m list)
+    then show ?thesis 
+    proof (cases x)
+      case (M1a b)
+      have "Max (Get1a ` set (known_msgs_acc st a)) < b"
+        using M1a \<open>a \<in> Q\<close> assms(1) local.Cons by fastforce
+      have "b \<in> Get1a ` set (known_msgs_acc st a)"
+        using M1a \<open>x \<in> set (known_msgs_acc st a)\<close> ballot_present by blast
+      have "b \<le> Max (set (map Get1a (known_msgs_acc st a)))"
+        using \<open>b \<in> Get1a ` set (known_msgs_acc st a)\<close> by auto
+      have "b \<le> Max (Get1a ` set (known_msgs_acc st a))"
+        using \<open>b \<le> Max (set (map Get1a (known_msgs_acc st a)))\<close> by auto
+      show ?thesis
+        using \<open>Max (Get1a ` set (known_msgs_acc st a)) < b\<close> \<open>b \<le> Max (Get1a ` set (known_msgs_acc st a))\<close> verit_comp_simplify1(3) by blast
+    next
+      case (M1b _ _)
+      then show ?thesis
+        using assms(2) by auto
+    next
+      case (M2a _ _ _)
+      then show ?thesis 
+        using assms(2) by auto
+    qed
+  qed
+qed
+
+
+
+(*
+There are four actions associated with AcceptorAction
+1. Process1a
+2. Process1b
+3. Process1bLearnerLoopStep
+4. Process1bLearnerLoopDone
+
+Under what conditions can these disable AcceptorAction?
+
+Preliminary hypotheses:
+
+Process1a will enable AcceptorAction if it queues a 1b message.
+If it's activated on a non-wellformed message, it may disable AcceptorAction 
+  if that's the last pending message
+  (Note: Proven)
+
+Process1b will enable AcceptorAction when the message is a max ballot because it
+  activates two_a_lrn_loop
+  (Note: Proven)
+
+Process1bLearnerLoopStep will maintain AcceptorAction since it doesn't disable two_a_lrn_loop
+  (Note: Proven)
+
+Process1bLearnerLoopDone may disable AcceptorAction if there are no messages left to proccess.
+  (Note: Proven)
+
+*)
+
+(*
+Note: 
+  Can the well-formedness condition be weakened?
+  Can it just be the wellformedness of m?
+*)
+lemma Process1a_Preserves_AcceptorAction:
+  assumes "Spec f"
+      and "Process1a a m (f i) (f (1 + i))"
+      and "WellFormed (f i) (M1b a (m # recent_msgs (f i) a)) \<or> 
+           (\<exists>m2 \<in> set (msgs (f i)). m2 \<noteq> m \<and> Recv_acc (f i) a m2 \<and> (type m2 = T1a \<or> type m2 = T1b))"
+    shows "Enabled (AcceptorAction a) (f (1 + i))"
+proof -
+  have qa: "AcceptorAction a (f i) (f (1 + i))"
+    by (metis Process1a.elims(2) Process1a_Next_Implies_AcceptorAction Process1a_Req_known_msgs Recv_acc.elims(2) Spec.elims(2) add_diff_cancel_left' assms(1) assms(2) plus_1_eq_Suc)
+  define st where "st = (f i)"
+  define st2 where "st2 = (f (1 + i))"
+  define new1b where "new1b = M1b a (m # recent_msgs st a)"
+  have "\<not> two_a_lrn_loop st2 a"
+    by (metis AcceptorAction.elims(2) Process1a.elims(2) Process1a_Not_Process1bLearnerLoopDone Process1a_Not_Process1bLearnerLoopStep Process1bLearnerLoop.simps assms(2) qa st2_def)
+  show ?thesis
+  proof (cases "WellFormed st new1b")
+    case True
+    have "Send new1b st st2
+          \<and> (recent_msgs st2 = (
+              \<lambda>a2. if a2 = a then []
+                             else recent_msgs st a2))
+          \<and> (queued_msg st2 = (
+              \<lambda>a2. if a2 = a then Some new1b 
+                             else queued_msg st a2))"
+      by (metis (full_types, opaque_lifting) Process1a.elims(2) True assms(2) new1b_def st2_def st_def)
+    have "type new1b = T1b"
+      using new1b_def by auto
+    have "WellFormed st2 new1b"
+      by (metis MessageType.distinct(5) True WellFormed.elims(1) \<open>type new1b = T1b\<close>)
+    have "ref new1b = {m} \<union> set (recent_msgs st a)"
+      using new1b_def by auto
+    have "m \<in> set (known_msgs_acc st2 a)"
+      using Process1a_Req_known_msgs assms(1) assms(2) diff_add_inverse st2_def by presburger
+    have "\<forall>m \<in> set (recent_msgs st a). m \<in> set (known_msgs_acc st a)"
+      by (metis AcceptorAction.elims(2) RecentMsgsSpec.elims(2) RecentMsgsSpecResult assms(1) qa st_def subset_code(1))
+    have "\<forall>m \<in> set (recent_msgs st a). m \<in> set (known_msgs_acc st2 a)"
+      using \<open>\<forall>m\<in>set (recent_msgs st a). m \<in> set (known_msgs_acc st a)\<close> assms(1) known_msgs_acc_preserved le_add2 st2_def st_def by blast
+    have "Proper_acc st2 a new1b"
+      by (simp add: \<open>\<forall>m\<in>set (recent_msgs st a). m \<in> set (known_msgs_acc st2 a)\<close> \<open>m \<in> set (known_msgs_acc st2 a)\<close> new1b_def)
+    have "new1b \<notin> set (known_msgs_acc st2 a)"
+      by (metis AcceptorAction.elims(2) KnownMsgs_accSpec.elims(2) KnownMsgs_accSpecResult Process1a.elims(2) Proper_acc.elims(2) Recv_acc.elims(2) Store_acc.elims(2) assms(1) assms(2) qa in_set_member member_rec(1) new1b_def ref.simps(2) st2_def)
+    have "Recv_acc st2 a new1b"
+      using Recv_acc.simps \<open>Proper_acc st2 a new1b\<close> \<open>WellFormed st2 new1b\<close> \<open>new1b \<notin> set (known_msgs_acc st2 a)\<close> by blast
+    show ?thesis
+      by (metis AcceptorAction.elims(2) AcceptorAction_NotEnabled \<open>Recv_acc st2 a new1b\<close> \<open>Send new1b st st2 \<and> recent_msgs st2 = (\<lambda>a2. if a2 = a then [] else recent_msgs st a2) \<and> queued_msg st2 = (\<lambda>a2. if a2 = a then Some new1b else queued_msg st a2)\<close> \<open>type new1b = T1b\<close> qa option.distinct(1) option.sel st2_def)
+  next
+    case False
+    have "(recent_msgs st2 = (
+              \<lambda>a2. if a2 = a then m # recent_msgs st a2 
+                             else recent_msgs st a2))
+          \<and> (msgs st = msgs st2)
+          \<and> (queued_msg st = queued_msg st2)"
+      by (metis (full_types, opaque_lifting) False Process1a.simps assms(2) new1b_def st2_def st_def)
+    have "queued_msg st2 a = None"
+      by (metis AcceptorAction.elims(2) Process1a_Not_Process1bLearnerLoopDone Process1a_Not_Process1bLearnerLoopStep Process1bLearnerLoop.simps Process1b_Not_Process1a \<open>recent_msgs st2 = (\<lambda>a2. if a2 = a then m # recent_msgs st a2 else recent_msgs st a2) \<and> msgs st = msgs st2 \<and> queued_msg st = queued_msg st2\<close> assms(2) qa st_def)
+    have "\<exists>m2 \<in> set (msgs st2). Recv_acc st2 a m2 \<and> (type m2 = T1a \<or> type m2 = T1b)"
+      by (smt (z3) False Process1a.simps Proper_acc.simps Recv_acc.simps Store_acc.elims(2) WellFormed_monotone assms(2) assms(3) list.set_intros(2) new1b_def set_ConsD st2_def st_def)
+    show ?thesis
+      by (metis AcceptorAction.elims(2) AcceptorAction_NotEnabled \<open>\<exists>m2\<in>set (msgs st2). Recv_acc st2 a m2 \<and> (type m2 = T1a \<or> type m2 = T1b)\<close> \<open>queued_msg st2 a = None\<close> qa st2_def)
+  qed
+qed
+
+lemma Process1a_Disables_AcceptorAction:
+  assumes "Spec f"
+      and "Process1a a m (f i) (f (1 + i))"
+      and "\<not> Enabled (AcceptorAction a) (f (1 + i))"
+    shows "\<not> WellFormed (f i) (M1b a (m # recent_msgs (f i) a))"
+      and "\<not> (\<exists>m2 \<in> set (msgs (f i)). m2 \<noteq> m \<and> Recv_acc (f i) a m2 \<and> (type m2 = T1a \<or> type m2 = T1b))"
+  using Process1a_Preserves_AcceptorAction assms(1) assms(2) assms(3) apply blast
+  using Process1a_Preserves_AcceptorAction assms(1) assms(2) assms(3) by blast  
+
+lemma Process1b_Preserves_AcceptorAction:
+  assumes "Spec f"
+      and "Process1b a m (f i) (f (1 + i))"
+      and "(\<forall> mb b :: Ballot. MaxBal (f i) a b \<and> B m b \<longrightarrow> mb \<le> b) \<or>
+           (\<exists>m2 \<in> set (msgs (f i)). m2 \<noteq> m \<and> Recv_acc (f i) a m2 \<and> (type m2 = T1a \<or> type m2 = T1b))"
+    shows "Enabled (AcceptorAction a) (f (1 + i))"
+proof -
+  define st where "st = f i"
+  define st2 where "st2 = f (1 + i)"
+  have qa: "AcceptorAction a st st2"
+    by (metis Process1b.elims(2) Process1b_Next_Implies_AcceptorAction Spec.elims(2) Suc_eq_plus1_left assms(1) assms(2) not_Cons_self st2_def st_def)
+  have "\<not> two_a_lrn_loop st a"
+    by (metis AcceptorAction.elims(2) Process1bLearnerLoop.simps Process1b_Not_Process1bLearnerLoopDone Process1b_Not_Process1bLearnerLoopStep assms(2) qa st2_def st_def)
+  then show ?thesis
+  proof (cases "\<forall> mb b :: Ballot. MaxBal (f i) a b \<and> B m b \<longrightarrow> mb \<le> b")
+    case True
+    have "two_a_lrn_loop st2 a"
+      sorry
+    then show ?thesis
+      by (metis AcceptorAction.elims(2) AcceptorAction_Enabled qa st2_def)
+  next
+    case False
+    have "\<not> two_a_lrn_loop st2 a"
+      sorry
+    have "queued_msg st2 a = None"
+      by (metis Process1b.elims(2) assms(2) st2_def)
+    have "\<exists>m2 \<in> set (msgs st). m2 \<noteq> m \<and> Recv_acc st a m2 \<and> (type m2 = T1a \<or> type m2 = T1b)"
+      using False assms(3) st_def by blast
+    then have "\<exists>m2 \<in> set (msgs st2). Recv_acc st2 a m2 \<and> (type m2 = T1a \<or> type m2 = T1b)"
+    proof (clarify)
+      fix m2
+      assume "m2 \<in> set (msgs st)"
+         and "m2 \<noteq> m"
+         and "Recv_acc st a m2"
+         and "type m2 = T1a \<or> type m2 = T1b"
+      have "m2 \<in> set (msgs st2)"
+        by (metis Process1b.elims(2) \<open>m2 \<in> set (msgs st)\<close> assms(2) st2_def st_def)
+      have "m2 \<notin> set (known_msgs_acc st2 a)"
+        by (metis Process1b.elims(2) Recv_acc.elims(2) Store_acc.elims(2) \<open>Recv_acc st a m2\<close> \<open>m2 \<noteq> m\<close> assms(2) in_set_member member_rec(1) st2_def st_def)
+      have "WellFormed st2 m2"
+        using Recv_acc.simps Wellformed_Conservation \<open>Recv_acc st a m2\<close> assms(1) le_add2 st2_def st_def by blast
+      have "Proper_acc st2 a m2"
+        sorry
+      have "Recv_acc st2 a m2"
+        using Recv_acc.simps \<open>Proper_acc st2 a m2\<close> \<open>WellFormed st2 m2\<close> \<open>m2 \<notin> set (known_msgs_acc st2 a)\<close> by blast
+      show ?thesis
+        using \<open>Recv_acc st2 a m2\<close> \<open>m2 \<in> set (msgs st2)\<close> \<open>type m2 = T1a \<or> type m2 = T1b\<close> by blast
+    qed
+    then show ?thesis
+      by (metis AcceptorAction.elims(2) AcceptorAction_NotEnabled \<open>queued_msg st2 a = None\<close> qa st2_def)
+  qed
+qed
+
+lemma Process1b_Disables_AcceptorAction:
+  assumes "Spec f"
+      and "Process1b a m (f i) (f (1 + i))"
+      and "\<not> Enabled (AcceptorAction a) (f (1 + i))"
+    shows "\<not> (\<forall> mb b :: Ballot. MaxBal (f i) a b \<and> B m b \<longrightarrow> mb \<le> b)"
+      and "\<not> (\<exists>m2 \<in> set (msgs (f i)). m2 \<noteq> m \<and> Recv_acc (f i) a m2 \<and> (type m2 = T1a \<or> type m2 = T1b))"
+  using Process1b_Preserves_AcceptorAction assms(1) assms(2) assms(3) apply blast
+  using Process1b_Preserves_AcceptorAction assms(1) assms(2) assms(3) by blast
+
+lemma Process1bLearnerLoopStep_Preserves_AcceptorAction:
+  assumes "Process1bLearnerLoopStep a ln st st2"
+      and "AcceptorAction a st st2"
+    shows "Enabled (AcceptorAction a) st2"
+proof -
+  have "two_a_lrn_loop st a"
+    by (meson AcceptorAction.elims(2) Process1a_Not_Process1bLearnerLoopStep Process1b_Not_Process1bLearnerLoopStep assms(1) assms(2))
+  then show ?thesis
+    by (metis AcceptorAction.elims(2) AcceptorAction_Enabled Process1bLearnerLoopStep.elims(2) assms(1) assms(2))
+qed
+
+lemma Process1bLearnerLoopDone_Preserves_AcceptorAction:
+  assumes "Spec f"
+      and "Process1bLearnerLoopDone a (f i) (f (1 + i))"
+      and "AcceptorAction a (f i) (f (1 + i))"
+      and "\<exists>m \<in> set (msgs (f i)). Recv_acc (f i) a m \<and> (type m = T1a \<or> type m = T1b)"
+    shows "Enabled (AcceptorAction a) (f (1 + i))"
+proof -
+  have "two_a_lrn_loop (f i) a"
+    by (meson AcceptorAction.elims(2) Process1a_Not_Process1bLearnerLoopDone Process1b_Not_Process1bLearnerLoopDone assms(2) assms(3))
+  have "queued_msg (f i) a = None"
+    using \<open>two_a_lrn_loop (f i) a\<close> assms(1) no_queue_during_loop by blast
+  have "queued_msg (f (1 + i)) a = None"
+    using \<open>queued_msg (f i) a = None\<close> assms(2) by auto
+  have "\<not> two_a_lrn_loop (f (1 + i)) a"
+    using assms(2) by auto
+  have "\<exists>m \<in> set (msgs (f (1 + i))). Recv_acc (f (1 + i)) a m \<and> (type m = T1a \<or> type m = T1b)"
+    using assms(2) assms(4) by auto
+  show ?thesis
+    by (meson AcceptorAction.elims(2) AcceptorAction_NotEnabled \<open>\<exists>m\<in>set (msgs (f (1 + i))). Recv_acc (f (1 + i)) a m \<and> (type m = T1a \<or> type m = T1b)\<close> \<open>queued_msg (f (1 + i)) a = None\<close> assms(3))
+qed
+
+lemma Process1bLearnerLoopDone_Disables_AcceptorAction:
+  assumes "Spec f"
+      and "Process1bLearnerLoopDone a (f i) (f (1 + i))"
+      and "AcceptorAction a (f i) (f (1 + i))"
+      and "\<not> Enabled (AcceptorAction a) (f (1 + i))"
+    shows "\<not> (\<exists>m \<in> set (msgs (f i)). Recv_acc (f i) a m \<and> (type m = T1a \<or> type m = T1b))"
+  using Process1bLearnerLoopDone_Preserves_AcceptorAction assms(1) assms(2) assms(3) assms(4) by blast
+
+lemma Process1bLearnerLoopDone_Preserves_AcceptorAction_INEQ:
+  assumes "Spec f"
+      and "Process1bLearnerLoopDone a (f i) (f (1 + i))"
+      and "f i \<noteq> f (1 + i)"
+      and "\<exists>m \<in> set (msgs (f i)). Recv_acc (f i) a m \<and> (type m = T1a \<or> type m = T1b)"
+    shows "Enabled (AcceptorAction a) (f (1 + i))"
+proof -
+  have qa: "AcceptorAction a (f i) (f (1 + i))"
+    by (metis Process1bLearnerLoopDone_Next_Implies_AcceptorAction Spec.elims(2) assms(1) assms(2) assms(3) plus_1_eq_Suc)
+  have "two_a_lrn_loop (f i) a"
+    by (meson AcceptorAction.elims(2) Process1a_Not_Process1bLearnerLoopDone Process1b_Not_Process1bLearnerLoopDone assms(2) qa)
+  have "queued_msg (f i) a = None"
+    using \<open>two_a_lrn_loop (f i) a\<close> assms(1) no_queue_during_loop by blast
+  have "queued_msg (f (1 + i)) a = None"
+    using \<open>queued_msg (f i) a = None\<close> assms(2) by auto
+  have "\<not> two_a_lrn_loop (f (1 + i)) a"
+    using assms(2) by auto
+  have "\<exists>m \<in> set (msgs (f (1 + i))). Recv_acc (f (1 + i)) a m \<and> (type m = T1a \<or> type m = T1b)"
+    using assms(2) assms(4) by auto
+  show ?thesis
+    by (meson AcceptorAction.elims(2) AcceptorAction_NotEnabled \<open>\<exists>m\<in>set (msgs (f (1 + i))). Recv_acc (f (1 + i)) a m \<and> (type m = T1a \<or> type m = T1b)\<close> \<open>queued_msg (f (1 + i)) a = None\<close> qa)
+qed
+
+lemma Preserves_AcceptorAction_Disabled_Three_Cases:
+  assumes "Spec f"
+      and "Enabled (AcceptorAction a) (f i)"
+      and "\<not> Enabled (AcceptorAction a) (f (1 + i))"
+    shows "(\<exists>m. Process1a a m (f i) (f (1 + i)) 
+              \<and> \<not> WellFormed (f i) (M1b a (m # recent_msgs (f i) a)) 
+              \<and> \<not> (\<exists>m2 \<in> set (msgs (f i)). m2 \<noteq> m \<and> Recv_acc (f i) a m2 \<and> (type m2 = T1a \<or> type m2 = T1b))) \<or>
+           (\<exists>m. Process1b a m (f i) (f (1 + i)) 
+              \<and> \<not> (\<forall> mb b :: Ballot. MaxBal (f i) a b \<and> B m b \<longrightarrow> mb \<le> b)
+              \<and> \<not> (\<exists>m2 \<in> set (msgs (f i)). m2 \<noteq> m \<and> Recv_acc (f i) a m2 \<and> (type m2 = T1a \<or> type m2 = T1b))) \<or>
+           (Process1bLearnerLoopDone a (f i) (f (1 + i)) 
+              \<and> \<not> (\<exists>m \<in> set (msgs (f i)). Recv_acc (f i) a m \<and> (type m = T1a \<or> type m = T1b)))"
+proof -
+  have "AcceptorAction a (f i) (f (1 + i))"
+    by (metis Spec.elims(2) Suc_eq_plus1_left assms(1) assms(2) assms(3) only_AcceptorAction_disables_AcceptorAction)
+  then have "(\<exists>m. Process1a a m (f i) (f (1 + i))) \<or>
+             (\<exists>m. Process1b a m (f i) (f (1 + i))) \<or>
+             Process1bLearnerLoopDone a (f i) (f (1 + i))"
+    by (meson AcceptorAction.elims(2) Process1bLearnerLoop.elims(2) Process1bLearnerLoopStep_Preserves_AcceptorAction assms(3))
+  then show ?thesis
+  proof (elim disjE)
+    assume "\<exists>m. Process1a a m (f i) (f (1 + i))"
+    then show ?thesis
+      using Process1a_Preserves_AcceptorAction assms(1) assms(3) by blast
+  next
+    assume "\<exists>m. Process1b a m (f i) (f (1 + i))"
+    then show ?thesis
+      by (metis Process1b_Preserves_AcceptorAction assms(1) assms(3))
+  next
+    assume "Process1bLearnerLoopDone a (f i) (f (1 + i))"
+    then show ?thesis
+      using Process1bLearnerLoopDone_Disables_AcceptorAction \<open>AcceptorAction a (f i) (f (1 + i))\<close> assms(1) assms(3) by presburger
+  qed
+qed
+
+
+
+end
